Some progress in program equivalence.

veric/semax_congruence.v
@@ -23,6 +23,16 @@ Require Import Coq.Classes.RelationClasses.
 Open Local Scope pred.
 Open Local Scope nat_scope.
 
+Lemma pred_ext'': forall {A} {agA: ageable A} (P Q: pred A),
+  (forall w: A, P w <-> Q w) <-> P = Q.
+Proof.
+  intros.
+  split; intros.
+  + apply pred_ext; intro w; rewrite H; auto.
+  + rewrite H.
+    reflexivity.
+Qed.
+
 Section extensions.
 Context (Espec : OracleKind).
 
@@ -35,6 +45,29 @@ Definition assert_safe_equiv c1 c2 :=
       assert_safe Espec gx vx tx (Kseq c1 :: k1) (construct_rho (filter_genv gx) vx tx) =
       assert_safe Espec gx vx tx (Kseq c2 :: k2) (construct_rho (filter_genv gx) vx tx)).
 
+Definition closed_wrt_modvars_equiv c1 c2 :=
+  forall F, closed_wrt_modvars c1 F <-> closed_wrt_modvars c2 F.
+
+Definition exit_tycon_equiv c1 c2 :=
+  forall Delta, exit_tycon c1 Delta = exit_tycon c2 Delta.
+
+Definition safeN__equiv c1 c2 :=
+  forall k1 k2,
+   (forall gx vx tx w,
+     (forall ora jm, m_phi jm = w ->
+        @safeN_ _ _ _ _ _ juicy_safety.Hrel (juicy_core_sem cl_core_sem) OK_spec
+          gx (level w) ora (State vx tx k1) jm) <->
+     (forall ora jm, m_phi jm = w ->
+        @safeN_ _ _ _ _ _ juicy_safety.Hrel (juicy_core_sem cl_core_sem) OK_spec
+          gx (level w) ora (State vx tx k2) jm)) ->
+   (forall gx vx tx w,
+     (forall ora jm, m_phi jm = w ->
+        @safeN_ _ _ _ _ _ juicy_safety.Hrel (juicy_core_sem cl_core_sem) OK_spec
+          gx (level w) ora (State vx tx (Kseq c1 :: k1)) jm) <->
+     (forall ora jm, m_phi jm = w ->
+        @safeN_ _ _ _ _ _ juicy_safety.Hrel (juicy_core_sem cl_core_sem) OK_spec
+          gx (level w) ora (State vx tx (Kseq c2 :: k2)) jm)).
+
 Definition modifiedvars_equiv c1 c2 :=
   forall S, modifiedvars' c1 S = modifiedvars' c2 S.
 
@@ -42,9 +75,94 @@ Definition update_tycon_equiv c1 c2 :=
   forall Delta, update_tycon Delta c1 = update_tycon Delta c2.
 
 Definition semax_equiv c1 c2 :=
-  assert_safe_equiv c1 c2 /\
+  safeN__equiv c1 c2 /\
   modifiedvars_equiv c1 c2 /\
   update_tycon_equiv c1 c2.
+
+Lemma safeN__assert_safe_equiv: forall c1 c2,
+  safeN__equiv c1 c2 -> assert_safe_equiv c1 c2.
+Proof.
+  unfold safeN__equiv, assert_safe_equiv.
+  intros.
+  specialize (H k1 k2).
+  apply pred_ext''; intros.
+  assert (forall (gx : genv) (vx : env) (tx : temp_env) w,
+       assert_safe Espec gx vx tx k1 (construct_rho (filter_genv gx) vx tx) w <->
+       assert_safe Espec gx vx tx k2 (construct_rho (filter_genv gx) vx tx) w).
+  Focus 1. {
+    clear - H0.
+    intros gx vx tx; specialize (H0 gx vx tx).
+    rewrite H0; tauto.
+  } Unfocus.
+  clear H0.
+
+  unfold assert_safe in H1 |- *.
+  simpl in H1 |- *.
+  split.
+
+  + unfold jsafeN, juicy_safety.safeN in H, H1 |- *.
+    intros.
+    apply H; clear H; [| intros; apply H0; auto | auto].
+    clear - H1.
+    intros; specialize (H1 gx vx tx w).
+    split; intros; apply H1; auto.
+  + unfold jsafeN, juicy_safety.safeN in H, H1 |- *.
+    intros.
+    apply H; clear H; [| intros; apply H0; auto | auto].
+    clear - H1.
+    intros; specialize (H1 gx vx tx w).
+    split; intros; apply H1; auto.
+Qed.
+
+Lemma modifiedvars_closed_wrt_modvars_equiv: forall c1 c2,
+  modifiedvars_equiv c1 c2 -> closed_wrt_modvars_equiv c1 c2.
+Proof.
+  unfold closed_wrt_modvars_equiv, modifiedvars_equiv.
+  unfold closed_wrt_modvars, modifiedvars.
+  intros.
+  rewrite H.
+  tauto.
+Qed.
+
+Lemma update_tycon_exit_tycon_equiv: forall c1 c2,
+  update_tycon_equiv c1 c2 -> exit_tycon_equiv c1 c2.
+Proof.
+  unfold update_tycon_equiv, exit_tycon_equiv.
+  intros.
+  extensionality ek.
+  destruct ek; auto.
+  simpl.
+  rewrite H; reflexivity.
+Qed.
+
+Lemma semax_equiv_spec: forall c1 c2,
+  semax_equiv c1 c2 ->
+  (forall P Q Delta, semax Espec Delta P c1 Q -> semax Espec Delta P c2 Q).
+Proof.
+  rewrite semax_unfold.
+  unfold semax_equiv.
+  intros ? ? [S_EQUIV [M_EQUIV U_EQUIV]] P Q Delta Hc1; intros.
+  specialize (Hc1 psi Delta' w TS Prog_OK k F).
+
+  apply modifiedvars_closed_wrt_modvars_equiv in M_EQUIV.
+  specialize (M_EQUIV F).
+  spec Hc1; [clear - M_EQUIV H; tauto |].
+
+  apply update_tycon_exit_tycon_equiv in U_EQUIV.
+  specialize (U_EQUIV Delta').
+  spec Hc1; [rewrite <- U_EQUIV in H0; auto |].
+
+  clear - S_EQUIV Hc1.
+  apply safeN__assert_safe_equiv in S_EQUIV.
+  unfold guard in Hc1 |- *.
+  intros te ve ? ? ? ? ?.
+  specialize (Hc1 te ve y H a' H0 H1).
+    (* This step uses that fact that current function has nothing to do with c1 and c2. *)
+  clear - S_EQUIV Hc1.
+  specialize (S_EQUIV k k (fun _ _ _ => eq_refl)).
+  rewrite <- S_EQUIV.
+  assumption.
+Qed.
 
 Lemma safeN_step_jsem_spec: forall gx vx tx n k ora jm,
   @safeN_ _ _ _ _ _ juicy_safety.Hrel (juicy_core_sem cl_core_sem) OK_spec
@@ -72,14 +190,35 @@ Proof.
     auto.
 Qed.
 
+(*
+Definition cl_step_equiv c1 c2 :=
+  forall k gx vx tx jm c' m',
+    cl_step gx (State vx tx (Kseq c1 :: k)) (m_dry jm) c' (m_dry m') <->
+    cl_step gx (State vx tx (Kseq c2 :: k)) (m_dry jm) c' (m_dry m').
+
+Lemma cl_step_safeN__equiv: forall c1 c2,
+  cl_step_equiv c1 c2 -> safeN__equiv c1 c2.
+Proof.
+  unfold cl_step_equiv, safeN__equiv.
+  intros.
+  pose proof H k1 gx vx tx.
+  pose proof H k2 gx vx tx.
+  clear H.
+  split; intros.
+  + specialize (H ora jm H3).
+    destruct (level w) as [| n]; [apply safeN_0 |].
+    rewrite !safeN_step_jsem_spec in H |- *.
+    destruct H as [c' [m' [? ?]]]; exists c', m'; (split; [| auto]).
+    rewrite H1 in H.
+*)
+
 Lemma safeN_step_jsem_seq: forall gx vx tx n c1 c2 k ora jm,
   @safeN_ _ _ _ _ _ juicy_safety.Hrel (juicy_core_sem cl_core_sem) OK_spec
-    gx (S n) ora (State vx tx (Kseq (Ssequence c1 c2) :: k)) jm =
+    gx (S n) ora (State vx tx (Kseq (Ssequence c1 c2) :: k)) jm <->
   @safeN_ _ _ _ _ _ juicy_safety.Hrel (juicy_core_sem cl_core_sem) OK_spec
     gx (S n) ora (State vx tx (Kseq c1 :: Kseq c2 :: k)) jm.
 Proof.
   intros.
-  apply prop_ext.
   rewrite !safeN_step_jsem_spec.
   split; intros; destruct H as [c' [m' [? ?]]]; exists c', m'; (split; [| auto]); clear H0.
   + inversion H; subst.
@@ -88,51 +227,28 @@ Proof.
     auto.
 Qed.
 
-Lemma pred_ext'': forall {A} {agA: ageable A} (P Q: pred A),
-  (forall w: A, P w <-> Q w) <-> P = Q.
+Lemma safeN__equiv_seq: forall c1 c2 c3 c4,
+  safeN__equiv c1 c2 ->
+  safeN__equiv c3 c4 ->
+  safeN__equiv (Ssequence c1 c3) (Ssequence c2 c4).
 Proof.
+  unfold safeN__equiv.
   intros.
-  split; intros.
-  + apply pred_ext; intro w; rewrite H; auto.
-  + rewrite H.
-    reflexivity.
-Qed.
-
-Lemma assert_safe_equiv_seq: forall c1 c2 c3 c4,
-  assert_safe_equiv c1 c2 ->
-  assert_safe_equiv c3 c4 ->
-  assert_safe_equiv (Ssequence c1 c3) (Ssequence c2 c4).
-Proof.
-  unfold assert_safe_equiv.
-  intros ? ? ? ? ?H ?H k1 k2.
   specialize (H (Kseq c3 :: k1) (Kseq c4 :: k2)).
   specialize (H0 k1 k2).
-
-  intro HH; specialize (H (H0 HH)); clear - H.
-  intros gx vx tx; specialize (H gx vx tx).
-  apply pred_ext''.
-  intros.
-  apply (proj2 (@pred_ext'' compcert_rmaps.R.rmap _ _ _)) with (w0 := w) in H.
-
-  unfold assert_safe in H |- *.
-  simpl in H |- *.
-  split; intros ? ? ? _ ?.
-
-  + unfold jsafeN, juicy_safety.safeN in H, H0 |- *.
-    destruct (level w) as [| n]; [apply safeN_0 |].
+  specialize (H (H0 H1)); clear - H.
+  specialize (H gx vx tx w).
+  split; intros.
+  + destruct (level w) as [| n]; [apply safeN_0 |].
     rewrite safeN_step_jsem_seq.
     apply H with (ora := ora) (jm := jm); auto; clear - H0.
-
-    intros ? ? _ ?.
+    intros.
     rewrite <- safeN_step_jsem_seq.
     apply H0; auto.
-
-  + unfold jsafeN, juicy_safety.safeN in H, H0 |- *.
-    destruct (level w) as [| n]; [apply safeN_0 |].
+  + destruct (level w) as [| n]; [apply safeN_0 |].
     rewrite safeN_step_jsem_seq.
     apply H with (ora := ora) (jm := jm); auto; clear - H0.
-
-    intros ? ? _ ?.
+    intros.
     rewrite <- safeN_step_jsem_seq.
     apply H0; auto.
 Qed.
@@ -168,94 +284,27 @@ Lemma semax_equiv_seq: forall c1 c2 c3 c4,
 Proof.
   unfold semax_equiv.
   intros.
-  repeat split.
-  + apply assert_safe_equiv_seq; tauto.
+  split; [| split].
+  + apply safeN__equiv_seq; tauto.
   + apply modifiedvars_equiv_seq; tauto.
   + apply update_tycon_equiv_seq; tauto.
 Qed.
-
-Lemma semax_equiv_spec: forall c1 c2,
-  semax_equiv c1 c2 ->
-  (forall P Q Delta, semax Espec Delta P c1 Q -> semax Espec Delta P c2 Q).
+(*
+Lemma Ssequence_assoc_assert_safe_equiv: forall c1 c2 c3,
+  safeN__equiv (Ssequence c1 (Ssequence c2 c3)) (Ssequence (Ssequence c1 c2) c3).
 Proof.
-  rewrite semax_unfold.
-  unfold semax_equiv, assert_safe_equiv, modifiedvars_equiv, update_tycon_equiv.
-  intros ? ? [A_EQUIV [M_EQUIV T_EQUIV]] P Q Delta Hc1; intros.
-  specialize (Hc1 psi Delta' w TS Prog_OK k F).
-  spec Hc1.
-  Focus 1. {
-    clear - H M_EQUIV.
-    unfold closed_wrt_modvars, modifiedvars in H |- *.
-    rewrite M_EQUIV.
-    assumption.
-  } Unfocus.
-  spec Hc1.
-  Focus 1. {
-    clear - H0 T_EQUIV.
-    replace (exit_tycon c1 Delta') with (exit_tycon c2 Delta'); [assumption |].
-    extensionality ek.
-    destruct ek; auto.
-    simpl.
-    rewrite T_EQUIV; reflexivity.
-  } Unfocus.
-  clear - A_EQUIV Hc1.
-  unfold guard in Hc1 |- *.
-  intros te ve ? ? ? ? ?.
-  specialize (Hc1 te ve y H a' H0 H1).
-    (* This step uses that fact that current function has nothing to do with c1 and c2. *)
-  clear - A_EQUIV Hc1.
-  specialize (A_EQUIV k k (fun _ _ _ => eq_refl)).
-  rewrite <- A_EQUIV.
-  assumption.
-Qed.
-
-
-
-
-Definition semax_stronger c1 c2 :=
-  (forall P Q Delta, semax Espec Delta P c1 Q -> semax Espec Delta P c2 Q) /\
-  (forall F, closed_wrt_modvars c2 F -> closed_wrt_modvars c1 F).
-
-Definition semax_equiv c1 c2 := forall P Q Delta,
-  semax Espec Delta P c1 Q = semax Espec Delta P c2 Q.
-
-Lemma closed_wrt_modvars_seq_left: forall c1 c2 c3 F,
-  (closed_wrt_modvars c2 F -> closed_wrt_modvars c1 F) ->
-  (closed_wrt_modvars (Ssequence c2 c3) F -> closed_wrt_modvars (Ssequence c1 c3) F).
-Admitted.
-
-Lemma split_and_right_first: forall (P Q: Prop), Q /\ (Q -> P) -> P /\ Q.
+  unfold safeN__equiv.
+  intros.
+  split; intros.
+  + destruct (level w) as [| n]; [apply safeN_0 |].
+    rewrite !safeN_step_jsem_seq.
+    
+Lemma Ssequence_assoc: forall c1 c2 c3,
+  semax_equiv (Ssequence c1 (Ssequence c2 c3)) (Ssequence (Ssequence c1 c2) c3).
 Proof.
   intros.
-  tauto.
-Qed.
+*)
+(*
 
-Check semax_unfold.
-Print guard.
-Print funassert.
-Print assert_safe.
-Print construct_rho.
-
-Lemma semax_equiv_seq_left: forall c1 c2 c3,
-  semax_stronger c1 c2 -> semax_stronger (Ssequence c1 c3) (Ssequence c2 c3).
-Proof.
-  unfold semax_stronger.
-  rewrite semax_unfold.
-  intros ? ? ? [?H Hclose].
-
-  (* Step 1 *)
-  apply split_and_right_first; split.
-  Focus 1. {
-    clear H.
-    intro F; specialize (Hclose F).
-    intro; eapply closed_wrt_modvars_seq_left; eauto.
-  } Unfocus.
-  intros.
-  specialize (H1 psi Delta' w TS Prog_OK k F (H0 F H2)).
-Print
-Print guard.
-  pose proof (fun P Q Delta
-  specialize (H P Q Delta).
-  intros.
 *)
 End extensions.
